path.v
@@ -3,7 +3,7 @@
 Require Import Utf8 PeanoNat Wf_nat List Lia.
 From larith Require Import tactics notations utilities.
 
-Section Graph_connectivity.
+Section Connecting_paths.
 
 Variable node : Type.
 Variable adj : node -> list node.
@@ -13,30 +13,30 @@ Hypothesis dec : ∀v w : node, {v = w} + {v ≠ w}.
 Hypothesis End_dec : ∀v, {End v} + {¬End v}.
 
 (* A path to an end node in graph g. *)
-Inductive path g : node -> Type :=
-  | path_stop v : End v -> path g v
-  | path_step v w : In w g -> In w (adj v) -> path g w -> path g v.
+Inductive path G : node -> Type :=
+  | path_stop v : End v -> path G v
+  | path_step v w : In w G -> In w (adj v) -> path G w -> path G v.
 
-Inductive Connected g v : Prop :=
-  | conn : path g v -> Connected g v.
+Inductive Connected G v : Prop :=
+  | conn : path G v -> Connected G v.
 
-Fixpoint path_length {g n} (p : path g n) : nat :=
+Fixpoint path_length {G n} (p : path G n) : nat :=
   match p with
   | path_stop _ _ _ => 0
   | path_step _ _ _ _ _ q => S (path_length q)
   end.
 
-Lemma path_subset g g' v :
-  path g' v -> (∀x, In x g' -> In x g) -> path g v.
+Lemma path_subset G H v :
+  path G v -> (∀x, In x G -> In x H) -> path H v.
 Proof.
 intros p subset; induction p.
 now apply path_stop. eapply path_step.
 apply subset, i. all: easy.
 Qed.
 
-Lemma Connected_split g g1 g2 v :
-  Connected g v -> (∀x, In x g <-> In x g1 \/ In x g2) ->
-  Exists (Connected g1) g2 \/ Connected g1 v.
+Lemma Connected_split G Ga Gb v :
+  Connected G v -> (∀x, In x G <-> In x Ga \/ In x Gb) ->
+  Exists (Connected Ga) Gb \/ Connected Ga v.
 Proof.
 intros [p] g_spec; induction p.
 - right; apply conn, path_stop, e.
@@ -47,31 +47,32 @@ intros [p] g_spec; induction p.
     easy. apply conn, X.
 Qed.
 
-Theorem Connected_dec g v :
-  {Connected g v} + {¬Connected g v}.
+(* We can effectively determine if v is connected to an end node. *)
+Theorem Connected_dec G v :
+  {Connected G v} + {¬Connected G v}.
 Proof.
-remember (length g) as n; revert Heqn; revert g v.
-apply lt_wf_rect with (n:=n); clear n; intros n IH g v g_len.
+remember (length G) as n; revert Heqn; revert G v.
+apply lt_wf_rect with (n:=n); clear n; intros n IH G v G_size.
 (* Check if v is a target state. *)
 destruct (End_dec v).
 left; apply conn, path_stop, e.
-(* Determine if there is an intersection between g and adj v. *)
-pose(gv := intersect dec g (adj v)).
-destruct (Nat.eq_dec (length gv) 0).
-- (* No path exists since g ∩ adj v = ∅. *)
+(* Determine if there is an intersection between G and adj v. *)
+pose(Gv := intersect dec G (adj v)).
+destruct (Nat.eq_dec (length Gv) 0).
+- (* No path exists since G ∩ adj v = ∅. *)
   right; intros [p]; inv p. apply in_nil with (a:=w).
   apply length_zero_iff_nil in e; rewrite <-e.
   now apply intersect_spec.
-- (* Show that g is not empty. *)
-  assert(length g ≠ 0). {
-    intros H; apply n1. unfold gv; rewrite intersect_length. lia. }
-  (* Determine if a node in g ∩ adj v is connected through g \ adj v. *)
-  pose(g' := subtract dec g (adj v)).
-  destruct (Exists_dec (Connected g') gv).
+- (* Show that G is not empty. *)
+  assert(length G ≠ 0). {
+    intros H; apply n1. unfold Gv; rewrite intersect_length. lia. }
+  (* Determine if a node in G ∩ adj v is connected through G \ adj v. *)
+  pose(G' := subtract dec G (adj v)).
+  destruct (Exists_dec (Connected G') Gv).
   + (* Decide using the induction hypothesis. *)
     intros; eapply IH. 2: reflexivity.
-    unfold g'; rewrite g_len, subtract_length.
-    fold gv; lia.
+    unfold G'; rewrite G_size, subtract_length.
+    fold Gv; lia.
   + (* A path exists. *)
     left. apply Exists_exists in e as [w [H1w [p]]].
     apply intersect_spec in H1w.
@@ -80,7 +81,7 @@ destruct (Nat.eq_dec (length gv) 0).
     intros; eapply subtract_spec, H0.
   + (* Any path would yield a contradiction. *)
     right. intros Hv; apply n2.
-    apply Connected_split with (g1:=g')(g2:=gv) in Hv as [Hv|[p]].
+    apply Connected_split with (Ga:=G')(Gb:=Gv) in Hv as [Hv|[p]].
     (* Either we find a path through g', or we find an impossible path. *)
     easy. exfalso; inv p. apply subtract_spec in H0; easy.
     (* Show that g = g1 ∪ g2. *)
@@ -93,7 +94,13 @@ destruct (Nat.eq_dec (length gv) 0).
       now apply intersect_spec in H0.
 Qed.
 
-End Graph_connectivity.
+(* A path can be shortened to at most the size of the graph. *)
+Theorem short_path G v (p : path G v) :
+  Σ q : path G v, path_length q <= length G.
+Proof.
+Admitted.
+
+End Connecting_paths.
 
 Arguments path {_}.
 Arguments path_length {_ _ _ _ _}.
